### Question:
Consider the terms of an arithmetic sequence: $-\frac{1}{3}, y+2, 4y, \ldots$. Solve for $y$.

### Answer:
For an arithmetic sequence, the difference between consecutive terms must be equal. Therefore, we can set up the following equations based on the sequence given:
\[ (y + 2) - \left(-\frac{1}{3}\right) = 4y - (y+2) \]

Simplify and solve these equations:
\[ y + 2 + \frac{1}{3} = 4y - y - 2 \]
\[ y + \frac{7}{3} = 3y - 2 \]
\[ \frac{7}{3} + 2 = 3y - y \]
\[ \frac{13}{3} = 2y \]
\[ y = \frac{13}{6} \]

Thus, the value of $y$ that satisfies the given arithmetic sequence is $\boxed{\frac{13}{6}}$.
### Question:
Suppose that $g(x) = 5x - 3$. What is $g^{-1}(g^{-1}(14))$?

### Answer:
First, we need to find the inverse function $g^{-1}(x)$. Given $g(x) = 5x - 3$, solve for $x$:
\[ y = 5x - 3 \]
\[ y + 3 = 5x \]
\[ x = \frac{y + 3}{5} \]
Thus, $g^{-1}(x) = \frac{x + 3}{5}$.

Now, apply $g^{-1}$ twice to the given value $14$:
\[ g^{-1}(14) = \frac{14 + 3}{5} = \frac{17}{5} \]
\[ g^{-1}\left(\frac{17}{5}\right) = \frac{\frac{17}{5} + 3}{5} = \frac{\frac{17}{5} + \frac{15}{5}}{5} = \frac{32}{5 \times 5} = \frac{32}{25} \]

Thus, $g^{-1}(g^{-1}(14)) = \boxed{\frac{32}{25}}$.